DivGadget.v
@@ -2,6 +2,7 @@ Require Import Metalib.Metatheory.
 From STLCZK Require Import Stlc.
 From STLCZK Require Import Gadgets.
 From STLCZK Require Import R1cs.
+From STLCZK Require Import GaloisField.
 
 Require Import Coqprime.elliptic.ZEll.
 Require Import Coq.Numbers.BinNums.
@@ -12,8 +13,9 @@ Import Z.
 Require Import Coq.ZArith.BinInt.
 
 Module DivGadget.
+  Include GaloisField.
   Include Gadgets.
-  Include R1cs.
+  Include R1csDep.
   (** Example 1: Division *)
   Definition div :=
     <{ \_: Field, (F1 / #0) }>.
@@ -26,58 +28,6 @@ Module DivGadget.
      }>.
 
   Compute normalize_all <{ div_check fp_one fp_one }>.
-  Ltac invert H := inversion H; subst; clear H.
-  Ltac invert_log_solved H g := 
-    solve [inversion H; fail; idtac "solved"] || invert H.
-
-  Lemma fp_mul_inv: forall n, n <> fp_zero -> pkmul (pkdiv fp_one n) n = fp_one.
-  Proof.
-    intros.
-    pose proof (pKfth p_prime) as FT.
-    invert FT.
-    rewrite Fdiv_def.
-    invert F_R.
-    rewrite <- Rmul_assoc.
-    rewrite Finv_l.
-    rewrite Rmul_1_l.
-    reflexivity.
-    assumption.
-  Qed.
-
-  Lemma fp_mul_div : forall n w, n <> fp_zero ->
-                               pkdiv (pkmul w n) n = w.
-  Proof.
-    intros.
-    pose proof (pKfth p_prime) as FT.
-    invert FT.
-    rewrite Fdiv_def.
-    invert F_R.
-    rewrite <- Rmul_assoc.
-    apply Finv_l in H.
-    replace (pkmul n (pkinv n)) with (pkmul (pkinv n) n) by (apply Rmul_comm).
-    rewrite H.
-    rewrite <- Rmul_comm.
-    rewrite Rmul_1_l.
-    reflexivity.
-  Qed.
-
-  Lemma fp_mul_zero_l: forall w, (pkmul w fp_zero) = fp_zero.
-  Proof.
-    intros.
-    cbn.
-    apply GZnZ.zirr.
-    
-    rewrite Zmult_comm.
-    pose proof (p_prime).
-    invert H.
-    rewrite Z.mod_0_l.
-    cbn.
-    reflexivity.    
-    intro Hcontra.    
-    rewrite Hcontra in H0.
-    invert H0.
-  Qed.
-
   Lemma neq_stlc_fp: forall n w, <{ fp n }> <> <{ fp w }> <-> n <> w.
   Proof.
     intro n.
@@ -89,19 +39,6 @@ Module DivGadget.
     - intro. invert H0; contradiction.
     - intro. invert H0; contradiction.
     - intro. invert H0; contradiction.
-  Qed.
-
-  Lemma mod_0_neq_1: 0 mod p <> 1 mod p.
-  Proof.
-    destruct (p_prime).
-    rewrite Z.mod_0_l.
-    rewrite Z.mod_1_l.
-    intro.
-    invert H1.
-    assumption.
-    intro.
-    rewrite H1 in H.
-    invert H.
   Qed.
 
   Ltac solve_stlc :=
